Require shard maps have no keys outside of shard domain
This strengthening of the invariant seems to be necessary to prove
encoding of shard install requests is safe.

src/program_proof/memkv/memkv_marshal_install_shard_proof.v
@@ -1,4 +1,4 @@
-From Perennial.program_proof Require Import grove_prelude.
+From Perennial.program_proof Require Import grove_prelude std_proof.
 From Goose.github_com.mit_pdos.gokv Require Import memkv.
 From Perennial.program_proof Require Export marshal_proof memkv.common_proof.
 
@@ -16,8 +16,29 @@ Record InstallShardRequestC := mkInstallShardC {
   IR_Kvs : gmap u64 (list u8)
 }.
 
-Definition has_encoding_InstallShardRequest (data:list u8) (args:InstallShardRequestC) : Prop.
-Admitted.
+Definition marshalledMapSize (m:gmap u64 (list u8)) : nat := 8 + 8 * 2 * (size m).
+
+Definition has_byte_map_encoding (m:gmap u64 (list u8)) (r:Rec) :=
+  ∃ l,
+  (int.Z (size m) = size m) ∧
+  NoDup l.*1 ∧
+  (list_to_map l) = m ∧
+  r = [EncUInt64 (size m)] ++ (EncUInt64 (size m) :: ((flat_map (λ u, [EncUInt64 u.1 ; EncBytes u.2]) l))).
+
+Definition has_encoding_InstallShardRequest (data:list u8) (args:InstallShardRequestC) : Prop :=
+  ∃ r, has_byte_map_encoding (args.(IR_Kvs)) r ∧
+       has_encoding data ([EncUInt64 args.(IR_CID); EncUInt64 args.(IR_Seq); EncUInt64 args.(IR_Sid)] ++ r).
+
+(*
+Definition has_encoding_InstallShardRequest (data:list u8) (args:InstallShardRequestC) : Prop :=
+  ∃ l,
+   let m := args.(IR_Kvs) in
+  (int.Z (size m) = size m) ∧
+  NoDup l.*1 ∧
+  (list_to_map l) = m ∧
+  has_encoding data ([EncUInt64 args.(IR_CID); EncUInt64 args.(IR_Seq); EncUInt64 args.(IR_Sid)] ++
+                    (EncUInt64 (size m) :: ((flat_map (λ u, [EncUInt64 u.1 ; EncBytes u.2]) l)))).
+*)
 
 Context `{!heapGS Σ}.
 
@@ -30,10 +51,149 @@ Definition own_InstallShardRequest args_ptr args : iProp Σ :=
   "HKvsMap" ∷ map.is_map kvs_ptr 1 (mv, (slice_val Slice.nil)) ∗
   "%HseqPositive" ∷ ⌜int.Z args.(IR_Seq) > 0⌝ ∗
   "Hvals" ∷ ([∗ set] k ∈ (fin_to_set u64),
-        ⌜shardOfC k ≠ args.(IR_Sid)⌝ ∨ (∃ q vsl, ⌜default (slice_val Slice.nil) (mv !! k) = (slice_val vsl)⌝ ∗ typed_slice.is_slice_small vsl byteT q (default [] (args.(IR_Kvs) !! k))) )
+        ⌜shardOfC k ≠ args.(IR_Sid) ∧ mv !! k = None ∧ args.(IR_Kvs) !! k = None⌝ ∨ (∃ q vsl, ⌜default (slice_val Slice.nil) (mv !! k) = (slice_val vsl)⌝ ∗ typed_slice.is_slice_small vsl byteT q (default [] (args.(IR_Kvs) !! k))) )
 .
 
-(* Pre: "HownShard" ∷ own_shard γ.(kv_gn) sid m *)
+(* TODO: need a hypothesis about correspondence between mv and m *)
+Lemma wp_EncSliceMap e mref mv m sz r remaining :
+marshalledMapSize m <= remaining →
+{{{
+    "HKvsMap" ∷ map.is_map mref 1 (mv, slice_val Slice.nil) ∗
+    "Henc" ∷ is_enc e sz r remaining
+}}}
+  EncSliceMap e #mref
+{{{
+     rmap, RET #();
+     ⌜has_byte_map_encoding m rmap⌝ ∗
+     map.is_map mref 1 (mv, slice_val Slice.nil) ∗
+     is_enc e sz (r ++ rmap) (remaining - marshalledMapSize m)
+}}}.
+Proof using Type*.
+Abort.
+(* TODO: this is copy + pasted from the old EncMap in kv_durable, probably hardly works *)
+(*
+  intros Hrem.
+  iIntros (Φ) "Hpre HΦ".
+  iNamed "Hpre".
+  wp_lam. wp_pures.
+
+  wp_apply (wp_MapLen with "Hmap").
+  iIntros "[%Hsize Hmap]".
+  unfold marshalledMapSize in Hrem.
+  wp_apply (wp_Enc__PutInt with "Henc").
+  { lia. }
+  iIntros "Henc".
+  wp_pures.
+  wp_apply (wp_MapIter_2 _ _ _ _ (EncMap_invariant e r sz (size m) (remaining - 8)) with "Hmap [Henc] [] [HΦ]").
+  {
+    iExists [] . iExists (remaining-8). simpl. iFrame.
+    iSplit.
+    { iPureIntro. apply NoDup_nil_2. }
+    iSplit; first done.
+    iPureIntro. split; first by lia.
+    replace (size ∅) with (0%nat).
+    { split; first by lia. apply map_disjoint_empty_r. }
+    symmetry. by apply map_size_empty_iff.
+  }
+  {
+    clear Φ.
+    iIntros (???? Φ) "!# [Hpre %Htodo] HΦ".
+    wp_pures.
+    iDestruct "Hpre" as (l rem' Hnodup Hl Hrem' Hremeq Hmdisjoint) "Henc".
+
+    assert (size mtodo ≠ 0%nat).
+    { apply map_size_non_empty_iff.
+      destruct (bool_decide (mtodo = ∅)) as [|] eqn:X.
+      { apply bool_decide_eq_true in X. rewrite X in Htodo. done. }
+      { by apply bool_decide_eq_false in X. }
+    }
+    wp_apply (wp_Enc__PutInt with "Henc").
+    {
+      lia.
+    }
+    iIntros "Henc".
+    wp_pures.
+
+    wp_apply (wp_Enc__PutInt with "Henc").
+    {
+      lia.
+    }
+    iIntros "Henc".
+    iApply "HΦ".
+    iExists (l ++ [(k, v)]), (rem' - 8 - 8).
+    iSplit.
+    { iPureIntro.
+      rewrite fmap_app.
+      rewrite NoDup_app.
+      split; first done.
+      split.
+      { intros.
+        simpl.
+        rewrite not_elem_of_cons.
+        split; last apply not_elem_of_nil.
+        destruct (decide (x = k)) as [->|]; last done.
+        exfalso.
+        apply elem_of_list_fmap_2 in H1 as [ [k0 v0] [Hk Hp]].
+        simpl in Hk.
+        eapply (elem_of_list_to_map_1 (M:=gmap _)) in Hnodup; eauto.
+        replace (list_to_map l) with (mdone) in Hnodup by eauto.
+        eapply map_disjoint_spec; eauto.
+        by rewrite Hk.
+      }
+      { apply NoDup_cons_2.
+        - apply not_elem_of_nil.
+        - apply NoDup_nil_2.
+      }
+    }
+    iSplit.
+    { iPureIntro.
+      rewrite -Hl.
+      apply list_to_map_snoc.
+      (* XXX: had to put the M there because typeclass resolution was not working well *)
+      rewrite (not_elem_of_list_to_map (M:=(@gmap u64 u64_eq_dec u64_countable))).
+      rewrite Hl.
+      destruct (mdone !! k) eqn:Hcase; last done.
+      exfalso; by eapply map_disjoint_spec.
+    }
+    iSplit.
+    { replace (size (delete k mtodo)) with (pred (size mtodo)).
+      { iPureIntro. lia. }
+      { symmetry. apply map_size_delete_Some. eauto. }
+    }
+    rewrite flat_map_app.
+    simpl.
+    replace ([EncUInt64 k; EncUInt64 v]) with ([EncUInt64 k] ++ [EncUInt64 v]) by eauto.
+    iFrame.
+    rewrite -app_assoc.
+    rewrite -app_assoc.
+    iFrame.
+    iPureIntro.
+
+    destruct (mdone !! k) eqn:X.
+    - exfalso. eapply map_disjoint_spec; eauto.
+    - split.
+      + rewrite map_size_insert_None; first lia. done.
+      + apply map_disjoint_insert_r_2.
+        { apply lookup_delete. }
+        by apply map_disjoint_delete_l.
+  }
+  iIntros "[Hmap Henc]".
+  iDestruct "Henc" as (l rem' Hnodup Hl _ ? ?) "Henc".
+  iApply ("HΦ" $! (
+              [EncUInt64 (size m)] ++
+              flat_map (λ u : u64 * u64, [EncUInt64 u.1; EncUInt64 u.2]) l)
+         ).
+  iFrame "Hmap".
+  unfold marshalledMapSize.
+  replace (remaining - (8 + 8 * 2 * size m)%nat) with (rem') by lia.
+  iFrame.
+  iPureIntro.
+  exists l.
+  rewrite -u64_Z_through_nat.
+  eauto.
+Qed.
+*)
+
 
 Lemma wp_encodeInstallShardRequest args_ptr args :
   {{{
@@ -46,6 +206,17 @@ Lemma wp_encodeInstallShardRequest args_ptr args :
                                                own_InstallShardRequest args_ptr args
   }}}.
 Proof.
+  iIntros (Φ) "Hpre HΦ".
+  iNamed "Hpre".
+  wp_lam.
+  wp_loadField.
+  wp_pures.
+  rewrite /SizeOfMarshalledMap.
+  (*
+  wp_apply (wp_SumAssumeNoOverflow).
+  iIntros (?) "Henc".
+  wp_pures.
+   *)
 Admitted.
 
 Lemma wp_decodeInstallShardRequest args args_sl argsData :
