src/program_proof/memkv/memkv_shard_definitions.v
@@ -225,7 +225,7 @@ Definition own_MemKVShardServer (s:loc) γ : iProp Σ :=
                       ⌜kvs_ptrs !! (int.nat sid) = Some kvs_ptr⌝ ∗
                       map.is_map kvs_ptr 1 (mv, (slice_val Slice.nil)) ∗
                       ([∗ set] k ∈ (fin_to_set u64),
-                       ⌜shardOfC k ≠ sid⌝ ∨ (∃ q vsl, ⌜default (slice_val Slice.nil) (mv !! k) = (slice_val vsl)⌝ ∗ typed_slice.is_slice_small vsl byteT q (default [] (m !! k))) )
+                       ⌜shardOfC k ≠ sid ∧ mv !! k = None ∧ m !! k = None ⌝ ∨ (∃ q vsl, ⌜default (slice_val Slice.nil) (mv !! k) = (slice_val vsl)⌝ ∗ typed_slice.is_slice_small vsl byteT q (default [] (m !! k))) )
                   )
                  ) ∗
   "HpeersMap" ∷ is_map (V:=loc) peers_ptr 1 peersM ∗
